[Lean] Generalize levels to any well order with unbounded successors

TT-model/example.lean
@@ -5,14 +5,81 @@ open Term
 @[simp]
 def idType k := (pi (lvl (lof k)) (pi (𝒰 (var 0)) (pi (var 0) (var 1))))
 
+-- idpoly : (j : Level< 69) → (A : 𝒰 j) → A → A
+-- idpoly ≔ λ j A x. x
+theorem idpoly : ⬝ ⊢ (abs (abs (abs (var 0)))) ∶ idType 69 := by
+  apply Wtf.abs (k := lof 69)
+  . apply Wtf.pi
+    . apply Wtf.lvl; apply Wtf.lof (k := 70); sorry; simp
+    . apply Wtf.pi
+      . apply Wtf.𝒰
+        apply Wtf.var
+        . sorry
+        . apply inHere; rfl
+      . apply Wtf.pi
+        . apply Wtf.sub
+          . apply Wtf.var
+            . sorry
+            . apply inThere; apply inHere; rfl; rfl
+          . apply Wtf.var
+            . sorry
+            . apply inHere; rfl
+        . apply Wtf.sub
+          . apply Wtf.var
+            . sorry
+            . apply inThere; apply inThere; apply inHere; rfl; rfl; rfl
+          . apply Wtf.var
+            . sorry
+            . apply inThere; apply inHere; rfl; rfl
+  . apply Wtf.abs
+    . apply Wtf.pi
+      . apply Wtf.𝒰
+        apply Wtf.var
+        . sorry
+        . apply inHere; rfl
+      . apply Wtf.pi
+        . apply Wtf.sub
+          . apply Wtf.var
+            . sorry
+            . apply inThere; apply inHere; rfl; rfl
+          . apply Wtf.var
+            . sorry
+            . apply inHere; rfl
+        . apply Wtf.sub
+          . apply Wtf.var
+            . sorry
+            . apply inThere; apply inThere; apply inHere; rfl; rfl; rfl
+          . apply Wtf.var
+            . sorry
+            . apply inThere; apply inHere; rfl; rfl
+    . apply Wtf.abs
+      . apply Wtf.pi
+        . apply Wtf.sub
+          . apply Wtf.var
+            . sorry
+            . apply inThere; apply inHere; rfl; rfl
+          . apply Wtf.var
+            . sorry
+            . apply inHere; rfl
+        . apply Wtf.sub
+          . apply Wtf.var
+            . sorry
+            . apply inThere; apply inThere; apply inHere; rfl; rfl; rfl
+          . apply Wtf.var
+            . sorry
+            . apply inThere; apply inHere; rfl; rfl
+      . apply Wtf.var
+        . sorry
+        . apply inHere; rfl
+
 -- idid : ((j : Level< (lof 4)) → (A : 𝒰 j) → A → A) → ((j : Level< (lof 3)) → (A : 𝒰 j) → A → A)
 -- idid ≔ λ id. id (lof 3) ((j : Level< (lof 3)) → (A : 𝒰 j) → A → A) (λ j. id j)
 -- All of the `sorry`s are boring proofs about context well formedness
-def idid : ⬝ ⊢ (abs (app (app ((app (var 0) (lof 3))) (idType 3)) (abs (app (var 1) (var 0))))) ∶ (pi (idType 4) (idType 3)) := by
+theorem idid : ⬝ ⊢ (abs (app (app ((app (var 0) (lof 3))) (idType 3)) (abs (app (var 1) (var 0))))) ∶ (pi (idType 4) (idType 3)) := by
   apply Wtf.abs (k := lof 4)
   . apply Wtf.pi
     . apply Wtf.pi
-      . apply Wtf.lvl; apply @Wtf.lof _ 4 5; sorry; omega
+      . apply Wtf.lvl; apply @Wtf.lof _ _ _ 5; sorry; simp
       . apply Wtf.pi
         . apply Wtf.𝒰
           apply Wtf.var
@@ -34,9 +101,9 @@ def idid : ⬝ ⊢ (abs (app (app ((app (var 0) (lof 3))) (idType 3)) (abs (app 
               . sorry
               . apply inThere; apply inHere; rfl; rfl
     . apply Wtf.sub
-      . apply @Wtf.lof _ 3; sorry; omega
+      . apply @Wtf.lof _ _ 3; sorry; simp
       . apply Wtf.pi
-        . apply Wtf.lvl; apply @Wtf.lof _ 3 4; sorry; omega
+        . apply Wtf.lvl; apply @Wtf.lof _ _ _ 4; sorry; simp
         . apply Wtf.pi
           . apply Wtf.𝒰
             apply Wtf.var
@@ -63,12 +130,11 @@ def idid : ⬝ ⊢ (abs (app (app ((app (var 0) (lof 3))) (idType 3)) (abs (app 
         . apply Wtf.var
           . sorry
           . apply inHere; rfl
-        . apply Wtf.lof; sorry; omega
+        . apply Wtf.lof; sorry; simp
         . simp; exact ⟨rfl, rfl⟩
       . apply Wtf.pi
         . apply Wtf.lvl
-          have lt : 3 < 4 := by omega
-          apply Wtf.lof _ lt; sorry
+          apply @Wtf.lof _ _ _ 4; sorry; simp
         . apply Wtf.pi
           . apply Wtf.𝒰
             apply Wtf.var
@@ -92,7 +158,7 @@ def idid : ⬝ ⊢ (abs (app (app ((app (var 0) (lof 3))) (idType 3)) (abs (app 
       . simp; exact ⟨rfl, rfl⟩
     . apply Wtf.abs (k := lof 3)
       . apply Wtf.pi
-        . apply Wtf.lvl; apply @Wtf.lof _ 3 4; sorry; omega
+        . apply Wtf.lvl; apply @Wtf.lof _ _ _ 4; sorry; simp
         . apply Wtf.pi
           . apply Wtf.𝒰
             apply Wtf.var
@@ -121,6 +187,6 @@ def idid : ⬝ ⊢ (abs (app (app ((app (var 0) (lof 3))) (idType 3)) (abs (app 
           . apply Wtf.var
             . sorry
             . apply inHere; rfl
-          . apply Wtf.lof; sorry; omega
+          . apply Wtf.lof; sorry; simp
         . simp
     . simp
