TT-model/semantics.lean
@@ -1,18 +1,20 @@
 import «TT-model».syntactics
 import «TT-model».reduction
 
-open Nat
+open LevelClass (L)
 open Term
 
 set_option autoImplicit false
 
-inductive Interp i (I : Nat → Term → Prop) : Term → (Term → Prop) → Prop where
+variable [lc : LevelClass]
+
+inductive Interp i (I : (j : L) → j < i → Term → Prop) : Term → (Term → Prop) → Prop where
   | pi a b Pa (Pf : Term → (Term → Prop) → Prop) :
     Interp i I a Pa →
     (∀ x, Pa x → ∃ Pb, Pf x Pb) →
     (∀ x Pb, Pf x Pb → Interp i I (subst (x +: var) b) Pb) →
     Interp i I (pi a b) (λ f ↦ ∀ x Pb, Pa x → Pf x Pb → Pb (app f x))
-  | 𝒰 j : j < i → Interp i I (𝒰 (lof j)) (I j)
+  | 𝒰 (j : L) (lt : j < i) : Interp i I (𝒰 (lof j)) (I j lt)
   | mty : Interp i I mty (λ _ ↦ False)
   | lvl k : Interp i I (lvl (lof k)) (λ a ↦ ∃ j, a ⇒⋆ lof j ∧ j < k)
   | step a b P :
@@ -21,12 +23,11 @@ inductive Interp i (I : Nat → Term → Prop) : Term → (Term → Prop) → Pr
     Interp i I a P
 notation:40 "⟦" a "⟧" i "," I "↘" P => Interp i I a P
 
-def Interps (i : Nat) : Term → (Term → Prop) → Prop :=
-  Interp i (λ j a ↦ if j < i then ∃ P, Interps j a P else False)
-notation:40 "⟦" a "⟧" i "↘" P => Interps i a P
+def Interps (i : L) : Term → (Term → Prop) → Prop :=
+  Interp i (λ j _ a ↦ ∃ P, Interps j a P)
+termination_by i
 
-theorem interp𝒰 {i I j P} : P = I j → j < i → ⟦ 𝒰 (lof j) ⟧ i , I ↘ P := by
-  intros e lt; subst e; constructor; assumption
+notation:40 "⟦" a "⟧" i "↘" P => Interps i a P
 
 /-*------------------------
   Simple inversion lemmas
@@ -56,14 +57,14 @@ theorem interpPiInv {i I a b P} (h : ⟦ pi a b ⟧ i , I ↘ P) :
         . apply parCong; apply parRefl; assumption
         . exact hb x Pb PfxPb
 
-theorem interp𝒰Inv {i I a P} (h : ⟦ 𝒰 a ⟧ i , I ↘ P) : ∃ j, a ⇒⋆ lof j ∧ j < i ∧ P = I j := by
+theorem interp𝒰Inv {i I a P} (h : ⟦ 𝒰 a ⟧ i , I ↘ P) : ∃ j lt, a ⇒⋆ lof j ∧ P = I j lt := by
   generalize e : 𝒰 a = b at h
   revert a; induction h
   all_goals intro a e; try contradiction
-  case 𝒰 j lt => injection e with e; subst e; exists j, Pars.refl _
+  case 𝒰 j lt => injection e with e; subst e; exists j, lt, Pars.refl _
   case step r _ ih => subst e; cases r; case 𝒰 r _ =>
     match ih rfl with
-    | ⟨j, r, lt, e⟩ => refine ⟨j, ?_, lt, e⟩; constructor <;> assumption
+    | ⟨j, lt, r, e⟩ => refine ⟨j, lt, ?_, e⟩; constructor <;> assumption
 
 theorem interpMtyInv {i I P} (h : ⟦ mty ⟧ i , I ↘ P) : P = (λ _ ↦ False) := by
   generalize e : mty = a at h
@@ -81,54 +82,26 @@ theorem interpLvlInv {i I a P} (h : ⟦ lvl a ⟧ i , I ↘ P) : ∃ k, a ⇒⋆
     match ih rfl with
     | ⟨k, r, e⟩ => refine ⟨k, ?_, e⟩; constructor <;> assumption
 
-/-*--------------------------------
-  Getting rid of the < in Interps
---------------------------------*-/
-
-theorem interpLtTo {i I a P} (h : ⟦ a ⟧ i , I ↘ P) :
-  ⟦ a ⟧ i , (λ j a ↦ if j < i then I j a else False) ↘ P := by
-  induction h <;> try (constructor <;> assumption)
-  case 𝒰 => apply interp𝒰; split <;> simp; assumption
-
-theorem interpLtFrom {i I a P}
-  (h : ⟦ a ⟧ i , (λ j a ↦ if j < i then I j a else False) ↘ P) :
-  ⟦ a ⟧ i , I ↘ P := by
-  induction h <;> try (constructor <;> assumption)
-  case 𝒰 => apply interp𝒰; split <;> simp; assumption
-
--- ⚠️ uses funext and propext ⚠️
-theorem interpLt i : Interps i = Interp i (λ j a ↦ ∃ P, ⟦ a ⟧ j ↘ P) := by
-  apply funext; intros; apply funext; intros; apply propext; constructor
-  . intro h; unfold Interps at h; apply interpLtFrom; exact h
-  . intro h; unfold Interps; apply interpLtTo; exact h
-
 /-*--------------------
   Better constructors
 --------------------*-/
-
-theorem interpPi {i I a b Pa P}
-  (ha : ⟦ a ⟧ i , I ↘ Pa)
-  (hb : ∀ x, Pa x → ∃ Pb, ⟦ subst (x +: var) b ⟧ i , I ↘ Pb) :
-  P = (λ f ↦ ∀ x Pb, Pa x → (⟦ subst (x +: var) b⟧ i , I ↘ Pb) → Pb (app f x)) →
-  ⟦ pi a b ⟧ i , I ↘ P := by
-  intro e; subst e; constructor; assumption; assumption; simp
 
 theorem interpsPi {i a b Pa P}
   (ha : ⟦ a ⟧ i ↘ Pa)
   (hb : ∀ x, Pa x → ∃ Pb, ⟦ subst (x +: var) b ⟧ i ↘ Pb) :
   P = (λ f ↦ ∀ x Pb, Pa x → (⟦ subst (x +: var) b⟧ i ↘ Pb) → Pb (app f x)) →
   ⟦ pi a b ⟧ i ↘ P := by
-  rw [interpLt] at *; apply interpPi ha hb
+  unfold Interps at *; intro e; subst e; constructor; assumption; assumption; simp
 
-theorem interps𝒰 {i j} (lt : j < i) :
+theorem interps𝒰 {i j : L} (lt : j < i) :
   ⟦ 𝒰 (lof j) ⟧ i ↘ (λ a ↦ ∃ P, ⟦ a ⟧ j ↘ P) := by
-  rw [interpLt]; apply interp𝒰 rfl lt
+  unfold Interps at *; constructor; assumption
 
 theorem interpsMty {i} : ⟦ mty ⟧ i ↘ (λ _ ↦ False) := by
-  rw [interpLt]; constructor
+  unfold Interps at *; constructor
 
 theorem interpsLvl {i k} : ⟦ lvl (lof k) ⟧ i ↘ (λ a ↦ ∃ j, a ⇒⋆ lof j ∧ j < k) := by
-  rw [interpLt]; constructor
+  unfold Interps at *; constructor
 
 /-*------------------------------------------------
   Interpretation respects conversion wrt the type
@@ -141,7 +114,7 @@ theorem interpFwd {i I a b P} (r : a ⇒ b) (h : ⟦ a ⟧ i , I ↘ P) : ⟦ b 
     . apply iha; assumption
     . assumption
     . intros; apply ihb; assumption; apply parCong; apply parRefl; assumption
-  case 𝒰 => cases r; case 𝒰 r => cases r; constructor; assumption
+  case 𝒰 => cases r; case 𝒰 r => cases r; constructor
   case mty => cases r; apply Interp.step <;> constructor
   case lvl => cases r; case lvl r => cases r; constructor
   case step r' _ ih =>
@@ -174,7 +147,7 @@ theorem interpsConv {i a b P} (r : a ⇔ b) (h : ⟦ a ⟧ i ↘ P) : ⟦ b ⟧ 
 ----------------------------------------------------*-/
 
 theorem interpsBwdsP {i a x y P} (r : x ⇒⋆ y) (h : ⟦ a ⟧ i ↘ P) : P y → P x := by
-  revert x y; rw [interpLt] at h; induction h
+  revert x y; unfold Interps at h; induction h
   case pi ihb =>
     intro _ _ r h x Pb Pax PfxPb
     exact ihb x Pb PfxPb (parsApp r (Pars.refl x)) (h x Pb Pax PfxPb)
@@ -212,7 +185,7 @@ theorem interpDet' {i I a P Q} (hP : ⟦ a ⟧ i , I ↘ P) (hQ : ⟦ a ⟧ i , 
           exact h x Pb' Pax' PfxPb'
   case 𝒰 =>
     match interp𝒰Inv hQ with
-    | ⟨j, r, _, e⟩ => injection (parsLofInv r) with ej; subst ej; simp [e]
+    | ⟨j, _, r, e⟩ => injection (parsLofInv r) with ej; subst ej; simp [e]
   case mty => simp [interpMtyInv hQ]
   case lvl =>
     match interpLvlInv hQ with
@@ -222,28 +195,25 @@ theorem interpDet' {i I a P Q} (hP : ⟦ a ⟧ i , I ↘ P) (hQ : ⟦ a ⟧ i , 
 theorem interpsDet' {i a P Q} (hP : ⟦ a ⟧ i ↘ P) (hQ : ⟦ a ⟧ i ↘ Q) : P = Q := by
   unfold Interps at *; apply interpDet' <;> assumption
 
-theorem interpCumul {i j I a P} : i ≤ j → (⟦ a ⟧ i , I ↘ P) → (⟦ a ⟧ j , I ↘ P) := by
-  intro lt h; revert j; induction h <;> intro j lt
+theorem interpsCumul {i j : L} {a P} (lt : i < j) (h : ⟦ a ⟧ i ↘ P) : ⟦ a ⟧ j ↘ P := by
+  revert j; unfold Interps at h; induction h
+  all_goals intro j lt; unfold Interps
   case pi iha ihb =>
     constructor
-    . exact iha lt
+    . unfold Interps at iha; exact iha lt
     . assumption
-    . intros; apply ihb <;> assumption
-  case 𝒰 => constructor; omega
+    . intros; unfold Interps at ihb; apply ihb <;> assumption
+  case 𝒰 k _ => constructor; apply IsTrans.trans <;> assumption
   case mty => constructor
   case lvl => constructor
-  case step ih => constructor; assumption; apply ih lt
+  case step ih => constructor; assumption; unfold Interps at ih; apply ih lt
 
-theorem interpsCumul {i j a P} : i ≤ j → (⟦ a ⟧ i ↘ P) → (⟦ a ⟧ j ↘ P) := by
-  rw [interpLt]; rw [interpLt]; apply interpCumul
-
+-- this is the only place we need trichotomy of <
 theorem interpsDet {i j a P Q} (hP : ⟦ a ⟧ i ↘ P) (hQ : ⟦ a ⟧ j ↘ Q) : P = Q := by
-  if i < j then
-    apply interpsDet' _ hQ
-    apply interpsCumul _ hP; omega
-  else
-    apply interpsDet' hP
-    apply interpsCumul _ hQ; omega
+  rcases IsTrichotomous.trichotomous (lt := lc.lt) i j with lt | eq | gt
+  . apply interpsDet' _ hQ; apply interpsCumul lt hP
+  . rw [eq] at hP; apply interpsDet' hP hQ
+  . apply interpsDet' hP; apply interpsCumul gt hQ
 
 /-*------------------------
   Better inversion lemmas
@@ -274,20 +244,19 @@ theorem interpsPiInv {i a b P} (h : ⟦ pi a b ⟧ i ↘ P) :
   ∃ Pa, (⟦ a ⟧ i ↘ Pa) ∧
     (∀ x, Pa x → ∃ Pb, ⟦ subst (x +: var) b ⟧ i ↘ Pb) ∧
     P = λ f ↦ ∀ x Pb, Pa x → (⟦ subst (x +: var) b⟧ i ↘ Pb) → Pb (app f x) := by
-  rw [interpLt] at *; apply interpPiInv' h
+  unfold Interps at *; apply interpPiInv' h
 
 theorem interps𝒰Inv {i a P} (h : ⟦ 𝒰 a ⟧ i ↘ P) :
   ∃ j, a ⇒⋆ lof j ∧ j < i ∧ P = λ a ↦ ∃ P, ⟦ a ⟧ j ↘ P := by
-  rw [interpLt] at h
-  apply interp𝒰Inv h
+  unfold Interps at h
+  match interp𝒰Inv h with
+  | ⟨j, lt, r, e⟩ => exact ⟨j, r, lt, e⟩
 
 theorem interpsMtyInv {i P} (h : ⟦ mty ⟧ i ↘ P) : P = (λ _ ↦ False) := by
-  rw [interpLt] at h
-  apply interpMtyInv h
+  unfold Interps at h; apply interpMtyInv h
 
 theorem interpsLvlInv {i a P} (h : ⟦ lvl a ⟧ i ↘ P) : ∃ k, a ⇒⋆ lof k ∧ P = (λ a ↦ ∃ j, a ⇒⋆ lof j ∧ j < k) := by
-  rw [interpLt] at h
-  apply interpLvlInv h
+  unfold Interps at h; apply interpLvlInv h
 
 /-*----------------
   Semantic typing
@@ -308,4 +277,4 @@ theorem semSubstCons {Γ : Ctxt} {σ i a A P} :
   intro hA ha hσ x B mem
   cases mem
   case here => rw [substRenamed]; exists i, P
-  case there B mem => rw [substRenamed]; apply hσ <;> assumption
+  case there B mem => rw [substRenamed]; apply hσ; assumption
