Main.lean
@@ -1,5 +1,7 @@
+import «TT-model».level
 import «TT-model».syntactics
 import «TT-model».reduction
 import «TT-model».typing
 import «TT-model».semantics
 import «TT-model».soundness
+import «TT-model».example
