TT-model/level.lean
@@ -1,0 +1,37 @@
+import Mathlib.Order.RelClasses
+
+/-*----------------------------------------------------------
+  Typeclass for levels and their required properties:
+  * Wellfoundedness is needed to build the logical relation
+  * Transitivity is needed for cumulativity of the LR
+  * Trichotomy is needed for determinism of the LR
+  * Lsucc is needed since every type has a type
+----------------------------------------------------------*-/
+
+class LevelClass where
+  L : Type
+  lt : L → L → Prop
+  wo : IsWellOrder L lt
+  lsucc i : ∃ j, lt i j
+open LevelClass
+
+infix:50 "<" => lt
+
+attribute [instance] wo
+
+instance [LevelClass] : WellFoundedRelation L :=
+  wo.toWellFoundedRelation
+
+/-*---------------------------------
+  The naturals are suitable levels
+---------------------------------*-/
+
+@[simp]
+instance LNat : LevelClass where
+  L := Nat
+  lt := LT.lt
+  wo := Nat.lt.isWellOrder
+  lsucc := λ i ↦ ⟨Nat.succ i, by omega⟩
+
+instance LOfNat : OfNat L n where
+  ofNat := n
